Proved pred_4_1_g_b_new

src/dvspec/dafny/att_spec_proofs/inv.dfy
@@ -1290,7 +1290,7 @@ module Att_Inv_With_Empty_Initial_Attestation_Slashing_DB
             ::
             slot < get_upperlimit_active_instances(n_state)
     }      
-
+    
     predicate pred_4_1_g_iii_b(dvn: DVState)    
     {
         forall hn |
@@ -1488,6 +1488,128 @@ module Att_Inv_With_Empty_Initial_Attestation_Slashing_DB
         forall i,j | 0 <= i < j < |n_state.attestation_duties_queue| :: n_state.attestation_duties_queue[i].slot <  n_state.attestation_duties_queue[j].slot           
     }
 
+    predicate inv_attestation_duty_queue_is_ordered_2_body_body(
+        dvn: DVState, 
+        n: BLSPubkey,
+        n_state: DVCNodeState
+    )
+    {
+        forall i, k, l, t  |
+            && 0 < i < |n_state.attestation_duties_queue|
+            && dvn.sequence_attestation_duties_to_be_served[k].node == n
+            && dvn.sequence_attestation_duties_to_be_served[l].node == n
+            && dvn.sequence_attestation_duties_to_be_served[t].node == n
+            && dvn.sequence_attestation_duties_to_be_served[k].attestation_duty.slot == n_state.attestation_duties_queue[i-1].slot
+            && dvn.sequence_attestation_duties_to_be_served[l].attestation_duty.slot == n_state.attestation_duties_queue[i].slot
+            ::
+            && k < l 
+            && !(k < t < l)
+
+    } 
+
+    predicate inv_attestation_duty_queue_is_ordered_3(dvn: DVState)    
+    {
+        forall hn |
+            && hn in dvn.honest_nodes_states.Keys          
+            ::
+            inv_attestation_duty_queue_is_ordered_3_body_body(
+                dvn, 
+                hn,
+                dvn.honest_nodes_states[hn]            
+            )                    
+    }     
+
+    predicate inv_attestation_duty_queue_is_ordered_3_body_body(
+        dvn: DVState, 
+        n: BLSPubkey,
+        n_state: DVCNodeState
+    )
+    {
+        forall i, k, l, t  |
+            inv_attestation_duty_queue_is_ordered_3_body_body_premise(
+                dvn,
+                n, 
+                n_state,
+                i,
+                k, 
+                l, 
+                t
+            )
+            ::
+            n_state.attestation_duties_queue[i-1].slot == dvn.sequence_attestation_duties_to_be_served[t].attestation_duty.slot
+
+    }       
+
+    predicate inv_attestation_duty_queue_is_ordered_3_body_body_premise(
+        dvn: DVState, 
+        n: BLSPubkey,
+        n_state: DVCNodeState,
+        i: nat, 
+        k: nat,
+        l: nat, 
+        t: nat
+    )
+    {
+            && 0 < i < |n_state.attestation_duties_queue|
+            && dvn.sequence_attestation_duties_to_be_served[k].node == n
+            && dvn.sequence_attestation_duties_to_be_served[l].node == n
+            && dvn.sequence_attestation_duties_to_be_served[t].node == n
+            && dvn.sequence_attestation_duties_to_be_served[k].attestation_duty.slot == n_state.attestation_duties_queue[i-1].slot
+            && dvn.sequence_attestation_duties_to_be_served[l].attestation_duty.slot == n_state.attestation_duties_queue[i].slot
+            && n_state.attestation_duties_queue[i-1].slot <= dvn.sequence_attestation_duties_to_be_served[t].attestation_duty.slot < dvn.sequence_attestation_duties_to_be_served[l].attestation_duty.slot 
+    } 
+        
+    predicate inv_attestation_duty_queue_is_ordered_4(dvn: DVState)    
+    {
+        forall hn |
+            && hn in dvn.honest_nodes_states.Keys          
+            ::
+            inv_attestation_duty_queue_is_ordered_4_body_body(
+                dvn, 
+                hn,
+                dvn.honest_nodes_states[hn],
+                dvn.index_next_attestation_duty_to_be_served
+            )                    
+    }           
+
+    predicate inv_attestation_duty_queue_is_ordered_4_body_body(
+        dvn: DVState, 
+        n: BLSPubkey,
+        n_state: DVCNodeState,
+        index_next_attestation_duty_to_be_served: nat
+    )  
+    {
+        |n_state.attestation_duties_queue| > 0 ==>
+            forall i |
+                inv_attestation_duty_queue_is_ordered_4_body_body_premise(
+                    dvn,
+                    n, 
+                    n_state,
+                    i,
+                    index_next_attestation_duty_to_be_served
+                )
+                ::
+                var last := n_state.attestation_duties_queue[|n_state.attestation_duties_queue|-1];
+                last.slot == dvn.sequence_attestation_duties_to_be_served[i].attestation_duty.slot 
+
+    }          
+
+    predicate inv_attestation_duty_queue_is_ordered_4_body_body_premise(
+        dvn: DVState, 
+        n: BLSPubkey,
+        n_state: DVCNodeState,
+        i: nat, 
+        index_next_attestation_duty_to_be_served: nat
+    )
+    requires |n_state.attestation_duties_queue| > 0
+    {
+            var last := n_state.attestation_duties_queue[|n_state.attestation_duties_queue|-1];
+            && i < index_next_attestation_duty_to_be_served
+            && dvn.sequence_attestation_duties_to_be_served[i].node == n
+            && last.slot <= dvn.sequence_attestation_duties_to_be_served[i].attestation_duty.slot 
+    }       
+         
+
     predicate inv_attestation_consensus_active_instances_keys_is_subset_of_att_slashing_db_hist(dvn: DVState)    
     {
         forall hn |
@@ -1528,186 +1650,245 @@ module Att_Inv_With_Empty_Initial_Attestation_Slashing_DB
         && n_state.current_attestation_duty.safe_get() == n_state.latest_attestation_duty.safe_get()
     }
 
-    // predicate inv_g_a(dvn: DVState)
-    // {
-    //     forall n | n in dvn.honest_nodes_states.Keys :: inv_g_a_body(dvn, n)
-    // }
+    predicate inv_g_a(dvn: DVState)
+    {
+        forall n | n in dvn.honest_nodes_states.Keys :: inv_g_a_body(dvn, n)
+    }
 
-    // predicate inv_g_a_body(
-    //     dvn: DVState, 
-    //     n: BLSPubkey
-    // )
-    // requires n in dvn.honest_nodes_states.Keys 
-    // {
-    //     var n_state := dvn.honest_nodes_states[n];
-    //     inv_g_a_body_body(dvn, n, n_state)
-    // }
+    predicate inv_g_a_body(
+        dvn: DVState, 
+        n: BLSPubkey
+    )
+    requires n in dvn.honest_nodes_states.Keys 
+    {
+        var n_state := dvn.honest_nodes_states[n];
+        inv_g_a_body_body(dvn, n, n_state)
+    }
 
-    // predicate inv_g_a_body_body(
-    //     dvn: DVState, 
-    //     n: BLSPubkey,
-    //     n_state: DVCNodeState
-    // )
-    // {
-    //     n_state.latest_attestation_duty.isPresent() ==>
-    //         forall an |
-    //             && an in dvn.sequence_attestation_duties_to_be_served.Values 
-    //             && an.node == n 
-    //             && an.attestation_duty.slot < n_state.latest_attestation_duty.safe_get().slot
-    //         ::
-    //             var slot := an.attestation_duty.slot;
-    //             && dvn.consensus_on_attestation_data[slot].decided_value.isPresent()
-    //             // && construct_SlashingDBAttestation_from_att_data(dvn.consensus_on_attestation_data[slot].decided_value.safe_get()) in n_state.attestation_slashing_db
-    // }         
+    predicate inv_g_a_body_body(
+        dvn: DVState, 
+        n: BLSPubkey,
+        n_state: DVCNodeState
+    )
+    {
+        n_state.latest_attestation_duty.isPresent() ==>
+            forall an |
+                && an in dvn.sequence_attestation_duties_to_be_served.Values 
+                && an.node == n 
+                && an.attestation_duty.slot < n_state.latest_attestation_duty.safe_get().slot
+            ::
+                var slot := an.attestation_duty.slot;
+                && dvn.consensus_on_attestation_data[slot].decided_value.isPresent()
+                // && construct_SlashingDBAttestation_from_att_data(dvn.consensus_on_attestation_data[slot].decided_value.safe_get()) in n_state.attestation_slashing_db
+    }         
 
-    // predicate inv_g_b_body_body(
-    //     dvn: DVState, 
-    //     n: BLSPubkey,
-    //     n_state: DVCNodeState
-    // )
-    // {
-    //     n_state.latest_attestation_duty.isPresent() ==>
-    //         forall an |
-    //             && an in dvn.sequence_attestation_duties_to_be_served.Values 
-    //             && an.node == n 
-    //             && an.attestation_duty.slot < n_state.latest_attestation_duty.safe_get().slot
-    //         ::
-    //             var slot := an.attestation_duty.slot;
-    //             && dvn.consensus_on_attestation_data[slot].decided_value.isPresent()
-    //             && construct_SlashingDBAttestation_from_att_data(dvn.consensus_on_attestation_data[slot].decided_value.safe_get()) in n_state.attestation_slashing_db
-    // } 
+    predicate inv_g_b_body_body(
+        dvn: DVState, 
+        n: BLSPubkey,
+        n_state: DVCNodeState
+    )
+    {
+        n_state.latest_attestation_duty.isPresent() ==>
+            forall an |
+                && an in dvn.sequence_attestation_duties_to_be_served.Values 
+                && an.node == n 
+                && an.attestation_duty.slot < n_state.latest_attestation_duty.safe_get().slot
+            ::
+                var slot := an.attestation_duty.slot;
+                && dvn.consensus_on_attestation_data[slot].decided_value.isPresent()
+                && construct_SlashingDBAttestation_from_att_data(dvn.consensus_on_attestation_data[slot].decided_value.safe_get()) in n_state.attestation_slashing_db
+    } 
 
-    // predicate inv_g_a_ii_body_body(
-    //     dvn: DVState, 
-    //     n: BLSPubkey,
-    //     n_state: DVCNodeState
-    // )
-    // {
-    //     (
-    //         &&  |n_state.attestation_duties_queue| > 0 
-    //         &&   !n_state.current_attestation_duty.isPresent()
-    //     )
-    //     ==>
-    //         forall an |
-    //             && an in dvn.sequence_attestation_duties_to_be_served.Values 
-    //             && an.node == n 
-    //             && an.attestation_duty.slot < n_state.attestation_duties_queue[0].slot
-    //         ::
-    //             var slot := an.attestation_duty.slot;
-    //             && dvn.consensus_on_attestation_data[slot].decided_value.isPresent()
-    //             // && construct_SlashingDBAttestation_from_att_data(dvn.consensus_on_attestation_data[slot].decided_value.safe_get()) in n_state.attestation_slashing_db
-    // }    
+    predicate inv_g_a_ii_body_body(
+        dvn: DVState, 
+        n: BLSPubkey,
+        n_state: DVCNodeState
+    )
+    {
+        (
+            &&  |n_state.attestation_duties_queue| > 0 
+            &&   !n_state.current_attestation_duty.isPresent()
+        )
+        ==>
+            forall an |
+                && an in dvn.sequence_attestation_duties_to_be_served.Values 
+                && an.node == n 
+                && an.attestation_duty.slot < n_state.attestation_duties_queue[0].slot
+            ::
+                var slot := an.attestation_duty.slot;
+                && dvn.consensus_on_attestation_data[slot].decided_value.isPresent()
+                // && construct_SlashingDBAttestation_from_att_data(dvn.consensus_on_attestation_data[slot].decided_value.safe_get()) in n_state.attestation_slashing_db
+    }    
 
-    // predicate inv_g_a_ii_a_body_body(
-    //     dvn: DVState, 
-    //     n: BLSPubkey,
-    //     n_state: DVCNodeState
-    // )
-    // {
-    //     (
-    //         &&  |n_state.attestation_duties_queue| > 0 
-    //         &&   !n_state.current_attestation_duty.isPresent()
-    //     )
-    //     ==>
-    //         forall an |
-    //             && an in dvn.sequence_attestation_duties_to_be_served.Values 
-    //             && an.node == n 
-    //             && an.attestation_duty.slot < n_state.attestation_duties_queue[0].slot
-    //         ::
-    //             var slot := an.attestation_duty.slot;
-    //             && dvn.consensus_on_attestation_data[slot].decided_value.isPresent()
-    //             && construct_SlashingDBAttestation_from_att_data(dvn.consensus_on_attestation_data[slot].decided_value.safe_get()) in n_state.attestation_slashing_db
-    // }        
+    predicate inv_g_a_ii_a(dvn: DVState)    
+    {
+        forall hn |
+            && hn in dvn.honest_nodes_states.Keys          
+            ::
+            inv_g_a_ii_a_body_body(
+                dvn, 
+                hn,
+                dvn.honest_nodes_states[hn]
+            )                    
+    }       
 
-    // predicate inv_g_a_iii_body_body(
-    //     dvn: DVState, 
-    //     n: BLSPubkey,
-    //     n_state: DVCNodeState,
-    //     index_next_attestation_duty_to_be_served: nat
-    // )
-    // {
-    //     (
-    //         &&  |n_state.attestation_duties_queue| == 0 
-    //         &&   !n_state.current_attestation_duty.isPresent()
-    //     ) ==>
-    //         forall i:nat  |
-    //             && i < index_next_attestation_duty_to_be_served
-    //             && var an := dvn.sequence_attestation_duties_to_be_served[i];
-    //             && an.node == n 
-    //             ::
-    //             && var an := dvn.sequence_attestation_duties_to_be_served[i];
-    //             var slot := an.attestation_duty.slot;
-    //             && dvn.consensus_on_attestation_data[slot].decided_value.isPresent()
-    // }            
+    predicate inv_g_a_ii_a_body_body(
+        dvn: DVState, 
+        n: BLSPubkey,
+        n_state: DVCNodeState
+    )
+    {
+        (
+            &&  |n_state.attestation_duties_queue| > 0 
+            &&   !n_state.current_attestation_duty.isPresent()
+        )
+        ==>
+            forall an |
+                && an in dvn.sequence_attestation_duties_to_be_served.Values 
+                && an.node == n 
+                && an.attestation_duty.slot < n_state.attestation_duties_queue[0].slot
+            ::
+                var slot := an.attestation_duty.slot;
+                && dvn.consensus_on_attestation_data[slot].decided_value.isPresent()
+                && construct_SlashingDBAttestation_from_att_data(dvn.consensus_on_attestation_data[slot].decided_value.safe_get()) in n_state.attestation_slashing_db
+    }     
+
+    predicate inv_g_a_iii(dvn: DVState)    
+    {
+        forall hn |
+            && hn in dvn.honest_nodes_states.Keys          
+            ::
+            inv_g_a_iii_body_body(
+                dvn, 
+                hn,
+                dvn.honest_nodes_states[hn],
+                dvn.index_next_attestation_duty_to_be_served
+            )                    
+    }          
+
+    predicate inv_g_a_iii_body_body(
+        dvn: DVState, 
+        n: BLSPubkey,
+        n_state: DVCNodeState,
+        index_next_attestation_duty_to_be_served: nat
+    )
+    {
+        (
+            &&  |n_state.attestation_duties_queue| == 0 
+            &&   !n_state.current_attestation_duty.isPresent()
+        ) ==>
+            forall i:nat  |
+                && i < index_next_attestation_duty_to_be_served
+                && var an := dvn.sequence_attestation_duties_to_be_served[i];
+                && an.node == n 
+                ::
+                && var an := dvn.sequence_attestation_duties_to_be_served[i];
+                var slot := an.attestation_duty.slot;
+                && dvn.consensus_on_attestation_data[slot].decided_value.isPresent()
+                && construct_SlashingDBAttestation_from_att_data(dvn.consensus_on_attestation_data[slot].decided_value.safe_get()) in n_state.attestation_slashing_db
+    }  
+
+    predicate inv_g_a_iv(dvn: DVState)    
+    {
+        forall hn |
+            && hn in dvn.honest_nodes_states.Keys          
+            ::
+            inv_g_a_iv_a_body_body(
+                dvn, 
+                hn,
+                dvn.honest_nodes_states[hn]
+            )                    
+    }     
+
+    predicate inv_g_a_iv_a_body_body(
+        dvn: DVState, 
+        n: BLSPubkey,
+        n_state: DVCNodeState
+    )
+    {
+        (
+            &&  |n_state.attestation_duties_queue| > 0 
+            &&   n_state.latest_attestation_duty.isPresent()
+        )
+        ==>
+            forall an |
+                && an in dvn.sequence_attestation_duties_to_be_served.Values 
+                && an.node == n 
+                && n_state.latest_attestation_duty.safe_get().slot < an.attestation_duty.slot < n_state.attestation_duties_queue[0].slot
+            ::
+                var slot := an.attestation_duty.slot;
+                && dvn.consensus_on_attestation_data[slot].decided_value.isPresent()
+                && construct_SlashingDBAttestation_from_att_data(dvn.consensus_on_attestation_data[slot].decided_value.safe_get()) in n_state.attestation_slashing_db
+    }                  
 
 
 
-    // predicate inv_g_c(dvn: DVState)
-    // {
-    //     forall n | n in dvn.honest_nodes_states.Keys :: inv_g_c_body(dvn, n)
-    // }    
+    predicate inv_g_c(dvn: DVState)
+    {
+        forall n | n in dvn.honest_nodes_states.Keys :: inv_g_c_body(dvn, n)
+    }    
 
-    // predicate inv_g_c_body(
-    //     dvn: DVState, 
-    //     n: BLSPubkey
-    // )
-    // requires n in dvn.honest_nodes_states.Keys 
-    // {
-    //     var n_state := dvn.honest_nodes_states[n];
-    //     inv_g_c_body_body(dvn, n, n_state, dvn.index_next_attestation_duty_to_be_served)
-    // }
+    predicate inv_g_c_body(
+        dvn: DVState, 
+        n: BLSPubkey
+    )
+    requires n in dvn.honest_nodes_states.Keys 
+    {
+        var n_state := dvn.honest_nodes_states[n];
+        inv_g_c_body_body(dvn, n, n_state, dvn.index_next_attestation_duty_to_be_served)
+    }
 
-    // predicate inv_g_c_body_body(
-    //     dvn: DVState, 
-    //     n: BLSPubkey,
-    //     n_state: DVCNodeState,
-    //     index_next_attestation_duty_to_be_served: nat
-    // )
-    // {
-    //     n_state.latest_attestation_duty.isPresent() ==>
-    //         forall i:nat  |
-    //             && i < index_next_attestation_duty_to_be_served
-    //             && var an := dvn.sequence_attestation_duties_to_be_served[i];
-    //             && an in dvn.sequence_attestation_duties_to_be_served.Values 
-    //             && an.node == n 
-    //             && an.attestation_duty.slot > n_state.latest_attestation_duty.safe_get().slot 
-    //             && !dvn.consensus_on_attestation_data[an.attestation_duty.slot].decided_value.isPresent()
-    //             ::
-    //             && var an := dvn.sequence_attestation_duties_to_be_served[i];
-    //             an.attestation_duty in n_state.attestation_duties_queue
-    // }    
+    predicate inv_g_c_body_body(
+        dvn: DVState, 
+        n: BLSPubkey,
+        n_state: DVCNodeState,
+        index_next_attestation_duty_to_be_served: nat
+    )
+    {
+        n_state.latest_attestation_duty.isPresent() ==>
+            forall i:nat  |
+                && i < index_next_attestation_duty_to_be_served
+                && var an := dvn.sequence_attestation_duties_to_be_served[i];
+                && an in dvn.sequence_attestation_duties_to_be_served.Values 
+                && an.node == n 
+                && an.attestation_duty.slot > n_state.latest_attestation_duty.safe_get().slot 
+                && !dvn.consensus_on_attestation_data[an.attestation_duty.slot].decided_value.isPresent()
+                ::
+                && var an := dvn.sequence_attestation_duties_to_be_served[i];
+                an.attestation_duty in n_state.attestation_duties_queue
+    }    
 
-    // predicate inv_g_c_ii_body_body(
-    //     dvn: DVState, 
-    //     n: BLSPubkey,
-    //     n_state: DVCNodeState,
-    //     index_next_attestation_duty_to_be_served: nat
-    // )
-    // {
-    //     !n_state.latest_attestation_duty.isPresent() ==>
-    //         forall i:nat  |
-    //             && i < index_next_attestation_duty_to_be_served
-    //             && var an := dvn.sequence_attestation_duties_to_be_served[i];
-    //             && an in dvn.sequence_attestation_duties_to_be_served.Values 
-    //             && an.node == n 
-    //             && !dvn.consensus_on_attestation_data[an.attestation_duty.slot].decided_value.isPresent()
-    //             ::
-    //             && var an := dvn.sequence_attestation_duties_to_be_served[i];
-    //             an.attestation_duty in n_state.attestation_duties_queue
-    // }    
+    predicate inv_g_c_ii_body_body(
+        dvn: DVState, 
+        n: BLSPubkey,
+        n_state: DVCNodeState,
+        index_next_attestation_duty_to_be_served: nat
+    )
+    {
+        !n_state.latest_attestation_duty.isPresent() ==>
+            forall i:nat  |
+                && i < index_next_attestation_duty_to_be_served
+                && var an := dvn.sequence_attestation_duties_to_be_served[i];
+                && an in dvn.sequence_attestation_duties_to_be_served.Values 
+                && an.node == n 
+                && !dvn.consensus_on_attestation_data[an.attestation_duty.slot].decided_value.isPresent()
+                ::
+                && var an := dvn.sequence_attestation_duties_to_be_served[i];
+                an.attestation_duty in n_state.attestation_duties_queue
+    }    
 
 
-    // predicate inv_g_d_body_body(
-    //     dvn: DVState, 
-    //     n: BLSPubkey,
-    //     n_state: DVCNodeState
-    // )
-    // {
-    //     forall slot |
-    //         && slot in n_state.future_att_consensus_instances_already_decided
-    //         ::
-    //         dvn.consensus_on_attestation_data[slot].decided_value.isPresent()
-    // }    
+    predicate inv_g_d_body_body(
+        dvn: DVState, 
+        n: BLSPubkey,
+        n_state: DVCNodeState
+    )
+    {
+        forall slot |
+            && slot in n_state.future_att_consensus_instances_already_decided
+            ::
+            dvn.consensus_on_attestation_data[slot].decided_value.isPresent()
+    }    
 
 
     /*
