src/dvspec/dafny/att_spec_proofs/ind_inv2.dfy
@@ -1,0 +1,1209 @@
+include "../commons.dfy"
+include "../att_spec_proofs/helper_sets_lemmas.dfy"
+include "../specification/dvc_spec.dfy"
+include "../specification/consensus.dfy"
+include "../specification/network.dfy"
+include "../specification/dvn.dfy"
+include "../att_spec_proofs/inv.dfy"
+include "dvn_next_inv.dfy"
+include "ind_inv.dfy"
+
+module Att_Ind_Inv_With_Empty_Initial_Attestation_Slashing_DB2
+{
+    import opened Types 
+    import opened CommonFunctions
+    import opened ConsensusSpec
+    import opened NetworkSpec
+    import opened DVCNode_Spec
+    import opened DV    
+    import opened Att_Inv_With_Empty_Initial_Attestation_Slashing_DB
+    import opened Helper_Sets_Lemmas
+    import opened DVN_Next_Inv
+    import opened Att_Ind_Inv_With_Empty_Initial_Attestation_Slashing_DB
+
+    lemma lemma_inv_attestation_duty_queue_is_ordered_3_body_body(
+        dvn: DVState, 
+        n: BLSPubkey,
+        n_state: DVCNodeState,
+        i: nat, 
+        k: nat,
+        l: nat, 
+        t: nat        
+    )
+    requires inv_attestation_duty_queue_is_ordered_3_body_body(dvn, n, n_state)
+    requires inv_attestation_duty_queue_is_ordered_3_body_body_premise(dvn, n, n_state, i, k, l, t)
+    ensures n_state.attestation_duties_queue[i-1].slot == dvn.sequence_attestation_duties_to_be_served[t].attestation_duty.slot
+    {
+
+    }
+
+    lemma lemma2_inv_attestation_duty_queue_is_ordered_3_body_body(
+        dvn: DVState, 
+        n: BLSPubkey,
+        n_state: DVCNodeState,
+        n'_state: DVCNodeState
+    )
+    requires inv_attestation_duty_queue_is_ordered_3_body_body(dvn, n , n_state)
+    requires n_state.attestation_duties_queue == n'_state.attestation_duties_queue
+    ensures inv_attestation_duty_queue_is_ordered_3_body_body(dvn, n , n'_state)
+    {
+        forall i: nat, k, l, t  |
+            inv_attestation_duty_queue_is_ordered_3_body_body_premise(
+                dvn,
+                n, 
+                n'_state,
+                i,
+                k, 
+                l, 
+                t
+            )
+        ensures 
+            n'_state.attestation_duties_queue[i-1].slot == dvn.sequence_attestation_duties_to_be_served[t].attestation_duty.slot      
+        {
+            // assert process.attestation_duties_queue != [];
+            assert i > 0;
+
+            assert inv_attestation_duty_queue_is_ordered_3_body_body_premise(
+                dvn,
+                n, 
+                n_state,
+                i,
+                k, 
+                l, 
+                t                        
+            );
+        }        
+    }
+
+    lemma  lemma_on_first_seq_element_elimination<T>(
+        s1: seq<T>,
+        s2: seq<T>,
+        i: nat
+    )
+    requires |s1| > 0 || s1 != []
+    requires s2 == s1[1..]
+    requires 0 <= i < |s2|
+    ensures s2[i] == s1[i+1]
+    {
+
+    }
+
+
+    lemma lemma_pred_4_1_b_new_f_serve_attestation_duty(
+        process: DVCNodeState,
+        attestation_duty: AttestationDuty,
+        s': DVCNodeState,
+        dvn: DVState,
+        n: BLSPubkey,
+        index_next_attestation_duty_to_be_served: nat
+    )
+    requires f_serve_attestation_duty.requires(process, attestation_duty)
+    requires s' == f_serve_attestation_duty(process, attestation_duty).state   
+    requires index_next_attestation_duty_to_be_served > 0    
+    requires inv_g_b_body_body_new(dvn, n, process)
+    requires inv_g_a_ii_a_body_body(dvn, n, process)
+    requires inv_g_a_iii_body_body(dvn, n, process, index_next_attestation_duty_to_be_served-1)
+    requires inv_g_iii_b_body_body(dvn, n, process, index_next_attestation_duty_to_be_served-1)
+    requires inv_g_d_a_body_body(dvn, n, process)
+    requires inv_attestation_duty_queue_is_ordered_3_body_body(dvn, n, process) 
+    requires inv_attestation_duty_queue_is_ordered_4_body_body(dvn, n, process, index_next_attestation_duty_to_be_served-1)  
+    requires is_sequence_attestation_duties_to_be_served_orderd(dvn);
+    requires 
+                var an' := dvn.sequence_attestation_duties_to_be_served[index_next_attestation_duty_to_be_served-1];
+                && an'.attestation_duty == attestation_duty
+                && an'.node == n
+    ensures inv_g_b_body_body_new(dvn, n, s');
+    {
+        var new_p := process.(
+                attestation_duties_queue := process.attestation_duties_queue + [attestation_duty],
+                all_rcvd_duties := process.all_rcvd_duties + {attestation_duty}
+        );
+
+        if |process.attestation_duties_queue| == 0 
+        {
+            assert inv_attestation_duty_queue_is_ordered_3_body_body(dvn, n, new_p);  
+        }
+        else 
+        {
+            forall i: nat, k, l, t  |
+                inv_attestation_duty_queue_is_ordered_3_body_body_premise(
+                    dvn,
+                    n, 
+                    new_p,
+                    i,
+                    k, 
+                    l, 
+                    t
+                )
+            ensures 
+                new_p.attestation_duties_queue[i-1].slot == dvn.sequence_attestation_duties_to_be_served[t].attestation_duty.slot      
+            {
+                // assert process.attestation_duties_queue != [];
+                assert i > 0;
+
+
+                if i != |new_p.attestation_duties_queue| - 1
+                {
+                    assert inv_attestation_duty_queue_is_ordered_3_body_body_premise(
+                        dvn,
+                        n, 
+                        process,
+                        i,
+                        k, 
+                        l, 
+                        t                        
+                    );
+                }
+                else 
+                {
+                    assert new_p.attestation_duties_queue[i-1] == process.attestation_duties_queue[|process.attestation_duties_queue|-1];
+
+                    assert l == index_next_attestation_duty_to_be_served-1;
+
+                    assert new_p.attestation_duties_queue[i-1].slot <= dvn.sequence_attestation_duties_to_be_served[t].attestation_duty.slot;
+
+                    assert inv_attestation_duty_queue_is_ordered_4_body_body_premise(dvn, n, process, t, index_next_attestation_duty_to_be_served-1);
+
+                    assert new_p.attestation_duties_queue[i-1].slot == dvn.sequence_attestation_duties_to_be_served[t].attestation_duty.slot;
+                }
+
+            }   
+        }
+
+
+
+        lemma_pred_4_1_b_new_f_check_for_next_queued_duty(new_p, s', dvn, n, index_next_attestation_duty_to_be_served);
+    }
+
+    lemma lemma_pred_4_1_b_new_f_att_consensus_decided(
+        process: DVCNodeState,
+        id: Slot,
+        decided_attestation_data: AttestationData,        
+        s': DVCNodeState,
+        dvn: DVState,
+        n: BLSPubkey,
+        index_next_attestation_duty_to_be_served: nat        
+    )
+    requires f_att_consensus_decided.requires(process, id, decided_attestation_data)
+    requires s' == f_att_consensus_decided(process, id, decided_attestation_data).state
+    requires inv_g_b_body_body_new(dvn, n, process)
+    requires inv_g_a_ii_a_body_body(dvn, n, process)
+    requires inv_g_a_iv_a_body_body(dvn, n, process)
+    requires inv_g_iii_b_body_body(dvn, n, process, index_next_attestation_duty_to_be_served)
+    requires inv_g_d_a_body_body(dvn, n, process)
+    requires inv_attestation_duty_queue_is_ordered_3_body_body(dvn, n, process)   
+    requires pred_inv_current_latest_attestation_duty_match_body_body(process)
+
+    requires dvn.consensus_on_attestation_data[id].decided_value.isPresent()
+    requires dvn.consensus_on_attestation_data[id].decided_value.safe_get() ==  decided_attestation_data 
+    ensures inv_g_b_body_body_new(dvn, n, s'); 
+    {
+        // TODO: Remove below by changing spec
+        assume id == process.current_attestation_duty.safe_get().slot;        
+        var local_current_attestation_duty := process.current_attestation_duty.safe_get();
+        var attestation_slashing_db := f_update_attestation_slashing_db(process.attestation_slashing_db, decided_attestation_data);
+
+        var fork_version := bn_get_fork_version(compute_start_slot_at_epoch(decided_attestation_data.target.epoch));
+        var attestation_signing_root := compute_attestation_signing_root(decided_attestation_data, fork_version);
+        var attestation_signature_share := rs_sign_attestation(decided_attestation_data, fork_version, attestation_signing_root, process.rs);
+        var attestation_with_signature_share := AttestationShare(
+                aggregation_bits := get_aggregation_bits(local_current_attestation_duty.validator_index),
+                data := decided_attestation_data, 
+                signature := attestation_signature_share
+            ); 
+
+        var s_mod := 
+            process.(
+                current_attestation_duty := None,
+                attestation_shares_to_broadcast := process.attestation_shares_to_broadcast[local_current_attestation_duty.slot := attestation_with_signature_share],
+                attestation_slashing_db := attestation_slashing_db,
+                attestation_consensus_engine_state := updateConsensusInstanceValidityCheck(
+                    process.attestation_consensus_engine_state,
+                    attestation_slashing_db
+                )
+            );
+
+        assert s_mod.attestation_duties_queue == process.attestation_duties_queue;
+
+        lemma2_inv_attestation_duty_queue_is_ordered_3_body_body(dvn, n, process, s_mod);
+
+        assert inv_g_b_body_body_new(dvn, n, s_mod);
+
+        assert get_upperlimit_decided_instances(s_mod) == process.latest_attestation_duty.safe_get().slot + 1;
+
+        if
+            &&  |s_mod.attestation_duties_queue| > 0 
+            &&   !s_mod.current_attestation_duty.isPresent()        
+        {
+            forall an |
+                && an in dvn.sequence_attestation_duties_to_be_served.Values 
+                && an.node == n 
+                && an.attestation_duty.slot < s_mod.attestation_duties_queue[0].slot   
+            ensures      
+                    var slot := an.attestation_duty.slot;
+                        && dvn.consensus_on_attestation_data[slot].decided_value.isPresent()
+                        && construct_SlashingDBAttestation_from_att_data(dvn.consensus_on_attestation_data[slot].decided_value.safe_get()) in s_mod.attestation_slashing_db
+                        ;                        
+            {
+                var slot := an.attestation_duty.slot;
+
+                if slot > s_mod.latest_attestation_duty.safe_get().slot
+                {
+                    assert 
+                        && dvn.consensus_on_attestation_data[slot].decided_value.isPresent()
+                        && construct_SlashingDBAttestation_from_att_data(dvn.consensus_on_attestation_data[slot].decided_value.safe_get()) in s_mod.attestation_slashing_db
+                        ;                    
+                }
+                else if slot == s_mod.latest_attestation_duty.safe_get().slot
+                {
+                    assert 
+                        && dvn.consensus_on_attestation_data[slot].decided_value.isPresent()
+                        && construct_SlashingDBAttestation_from_att_data(dvn.consensus_on_attestation_data[slot].decided_value.safe_get()) in s_mod.attestation_slashing_db
+                        ;                         
+                }
+                else 
+                {
+                    assert slot < s_mod.latest_attestation_duty.safe_get().slot;
+                    assert 
+                        && dvn.consensus_on_attestation_data[slot].decided_value.isPresent()
+                        && construct_SlashingDBAttestation_from_att_data(dvn.consensus_on_attestation_data[slot].decided_value.safe_get()) in s_mod.attestation_slashing_db
+                        ;                           
+                }
+
+            }
+        }
+        assert inv_g_a_ii_a_body_body(dvn, n, s_mod);
+
+
+        lemma_pred_4_1_b_new_f_check_for_next_queued_duty(s_mod, s', dvn, n, index_next_attestation_duty_to_be_served);             
+    }  
+
+    lemma lemma_f_listen_for_new_imported_blocks_helper_1(
+        dvn: DVState,
+        process: DVCNodeState,
+        block: BeaconBlock,
+        new_consensus_instances_already_decided: map<Slot, AttestationData>
+    )
+    requires f_listen_for_new_imported_blocks_helper_1.requires(process, block)
+    requires new_consensus_instances_already_decided == f_listen_for_new_imported_blocks_helper_1(process, block)
+    requires pred_4_1_b(dvn)
+    requires pred_4_1_c(dvn)
+    ensures 
+        forall slot | 
+                slot in new_consensus_instances_already_decided
+                :: 
+                && dvn.consensus_on_attestation_data[slot].decided_value.isPresent()
+                && dvn.consensus_on_attestation_data[slot].decided_value.safe_get() == new_consensus_instances_already_decided[slot]
+                ;  
+    {
+        forall slot | slot in new_consensus_instances_already_decided
+        ensures 
+            && dvn.consensus_on_attestation_data[slot].decided_value.isPresent()
+            && dvn.consensus_on_attestation_data[slot].decided_value.safe_get() == new_consensus_instances_already_decided[slot]
+            ;         
+        {
+
+            var valIndex := bn_get_validator_index(process.bn, block.body.state_root, process.dv_pubkey);
+
+
+            var a :| 
+                && a in block.body.attestations
+                && isMyAttestation(a, process, block, valIndex)
+                && a.data == new_consensus_instances_already_decided[slot]
+            ;
+
+            var an :| assume
+                && an in dvn.honest_nodes_states.Keys 
+                && a in dvn.honest_nodes_states[an].bn.attestations_submitted
+                
+                ;
+
+            var hn', att_share: AttestationShare :| pred_4_1_b_exists(dvn, hn', att_share, a);
+
+            assert
+            && dvn.consensus_on_attestation_data[att_share.data.slot].decided_value.isPresent()
+            && dvn.consensus_on_attestation_data[att_share.data.slot].decided_value.safe_get() == att_share.data;
+
+            // assert slot in process.future_att_consensus_instances_already_decided;
+            assert
+            && dvn.consensus_on_attestation_data[slot].decided_value.isPresent()
+            && dvn.consensus_on_attestation_data[slot].decided_value.safe_get() == new_consensus_instances_already_decided[slot]
+            ;              
+        }
+    }
+
+
+    lemma lemma_pred_4_1_b_new_f_listen_for_new_imported_blocks(
+        process: DVCNodeState,
+        block: BeaconBlock,
+        s': DVCNodeState,
+        dvn: DVState,
+        n: BLSPubkey,
+        index_next_attestation_duty_to_be_served: nat        
+    )
+    requires f_listen_for_new_imported_blocks.requires(process, block)
+    requires s' == f_listen_for_new_imported_blocks(process, block).state       
+    requires inv_g_b_body_body_new(dvn, n, process)
+    requires inv_g_a_ii_a_body_body(dvn, n, process)
+    requires inv_g_iii_b_body_body(dvn, n, process, index_next_attestation_duty_to_be_served)
+    requires inv_g_d_a_body_body(dvn, n, process)
+    requires inv_attestation_duty_queue_is_ordered_3_body_body(dvn, n, process) 
+    requires pred_inv_current_latest_attestation_duty_match_body_body(process)
+    requires pred_4_1_b(dvn)
+    requires pred_4_1_c(dvn)
+    requires inv_g_a_iv_a_body_body(dvn, n, process)
+    ensures inv_g_b_body_body_new(dvn, n, s');
+    {
+        var new_consensus_instances_already_decided := f_listen_for_new_imported_blocks_helper_1(process, block);
+
+        var att_consensus_instances_already_decided := process.future_att_consensus_instances_already_decided + new_consensus_instances_already_decided;
+
+        var future_att_consensus_instances_already_decided := 
+            f_listen_for_new_imported_blocks_helper_2(process, att_consensus_instances_already_decided);
+
+        var new_process :=
+                process.(
+                    future_att_consensus_instances_already_decided := future_att_consensus_instances_already_decided,
+                    attestation_consensus_engine_state := stopConsensusInstances(
+                                    process.attestation_consensus_engine_state,
+                                    att_consensus_instances_already_decided.Keys
+                    ),
+                    attestation_shares_to_broadcast := process.attestation_shares_to_broadcast - att_consensus_instances_already_decided.Keys,
+                    rcvd_attestation_shares := process.rcvd_attestation_shares - att_consensus_instances_already_decided.Keys                    
+                );                     
+
+        if new_process.current_attestation_duty.isPresent() && new_process.current_attestation_duty.safe_get().slot in att_consensus_instances_already_decided
+        {
+            // Stop(current_attestation_duty.safe_get().slot);
+            var decided_attestation_data := att_consensus_instances_already_decided[new_process.current_attestation_duty.safe_get().slot];
+            var new_attestation_slashing_db := f_update_attestation_slashing_db(new_process.attestation_slashing_db, decided_attestation_data);
+            var s_mod := new_process.(
+                current_attestation_duty := None,
+                attestation_slashing_db := new_attestation_slashing_db,
+                attestation_consensus_engine_state := updateConsensusInstanceValidityCheck(
+                    new_process.attestation_consensus_engine_state,
+                    new_attestation_slashing_db
+                )                
+            );
+
+            lemma2_inv_attestation_duty_queue_is_ordered_3_body_body(dvn, n, process, s_mod);
+
+
+            lemma_f_listen_for_new_imported_blocks_helper_1(
+                dvn,
+                process,
+                block,
+                new_consensus_instances_already_decided
+            );
+
+            assert 
+                && dvn.consensus_on_attestation_data[new_process.current_attestation_duty.safe_get().slot].decided_value.isPresent()
+                && dvn.consensus_on_attestation_data[new_process.current_attestation_duty.safe_get().slot].decided_value.safe_get() == decided_attestation_data
+            ;                        
+
+            assert inv_g_d_a_body_body(dvn, n, s_mod);                  
+
+            assert inv_g_b_body_body_new(dvn, n, s_mod);
+
+
+            if
+                &&  |s_mod.attestation_duties_queue| > 0 
+                &&   !s_mod.current_attestation_duty.isPresent()        
+            {
+                forall an |
+                    && an in dvn.sequence_attestation_duties_to_be_served.Values 
+                    && an.node == n 
+                    && an.attestation_duty.slot < s_mod.attestation_duties_queue[0].slot   
+                ensures      
+                        var slot := an.attestation_duty.slot;
+                            && dvn.consensus_on_attestation_data[slot].decided_value.isPresent()
+                            && construct_SlashingDBAttestation_from_att_data(dvn.consensus_on_attestation_data[slot].decided_value.safe_get()) in s_mod.attestation_slashing_db
+                            ;                        
+                {
+                    var slot := an.attestation_duty.slot;
+
+                    if slot > s_mod.latest_attestation_duty.safe_get().slot
+                    {
+                        assert 
+                            && dvn.consensus_on_attestation_data[slot].decided_value.isPresent()
+                            && construct_SlashingDBAttestation_from_att_data(dvn.consensus_on_attestation_data[slot].decided_value.safe_get()) in s_mod.attestation_slashing_db
+                            ;                    
+                    }
+                    else if slot == s_mod.latest_attestation_duty.safe_get().slot
+                    {
+                        assert 
+                            && dvn.consensus_on_attestation_data[slot].decided_value.isPresent()
+                            && construct_SlashingDBAttestation_from_att_data(dvn.consensus_on_attestation_data[slot].decided_value.safe_get()) in s_mod.attestation_slashing_db
+                            ;                         
+                    }
+                    else 
+                    {
+                        assert slot < s_mod.latest_attestation_duty.safe_get().slot;
+                        assert 
+                            && dvn.consensus_on_attestation_data[slot].decided_value.isPresent()
+                            && construct_SlashingDBAttestation_from_att_data(dvn.consensus_on_attestation_data[slot].decided_value.safe_get()) in s_mod.attestation_slashing_db
+                            ;                           
+                    }
+
+                }
+            }
+            assert inv_g_a_ii_a_body_body(dvn, n, s_mod);                 
+
+            forall an |
+                && an in dvn.sequence_attestation_duties_to_be_served.Values 
+                && an.node == n 
+                && an.attestation_duty.slot < get_upperlimit_decided_instances(s_mod)
+            {
+                if an.attestation_duty.slot < get_upperlimit_decided_instances(process)
+                {
+
+                }
+                else 
+                {
+                    assert an.attestation_duty.slot == new_process.current_attestation_duty.safe_get().slot;
+                }
+            }            
+
+            
+            lemma_pred_4_1_b_new_f_check_for_next_queued_duty(s_mod, s', dvn, n, index_next_attestation_duty_to_be_served);                    
+        }        
+    }      
+    
+    
+    // lemma lemma_pred_4_1_b_new_f_check_for_next_queued_duty_fake(
+    //     process: DVCNodeState,
+    //     s': DVCNodeState,
+    //     dvn: DVState,
+    //     n: BLSPubkey,
+    //     index_next_attestation_duty_to_be_served: nat
+    // )
+    // requires f_check_for_next_queued_duty.requires(process)
+    // requires s' == f_check_for_next_queued_duty(process).state   
+    // requires inv_g_b_body_body_new(dvn, n, process)
+    // requires inv_g_a_ii_a_body_body(dvn, n, process)
+    // requires inv_g_iii_b_body_body(dvn, n, process, index_next_attestation_duty_to_be_served)
+    // // requires inv_g_d_a_body_body(dvn, n, process)
+    // requires inv_attestation_duty_queue_is_ordered_3_body_body(dvn, n, process)  
+
+    // ensures inv_g_b_body_body_new(dvn, n, s');
+    // decreases process.attestation_duties_queue    
+    
+    lemma lemma_pred_4_1_b_new_f_check_for_next_queued_duty(
+        process: DVCNodeState,
+        s': DVCNodeState,
+        dvn: DVState,
+        n: BLSPubkey,
+        index_next_attestation_duty_to_be_served: nat
+    )
+    requires f_check_for_next_queued_duty.requires(process)
+    requires s' == f_check_for_next_queued_duty(process).state   
+    requires inv_g_b_body_body_new(dvn, n, process)
+    requires inv_g_a_ii_a_body_body(dvn, n, process)
+    requires inv_g_iii_b_body_body(dvn, n, process, index_next_attestation_duty_to_be_served)
+    requires inv_g_d_a_body_body(dvn, n, process)
+    requires inv_attestation_duty_queue_is_ordered_3_body_body(dvn, n, process)  
+
+    ensures inv_g_b_body_body_new(dvn, n, s');
+    decreases process.attestation_duties_queue
+    {
+        if  && process.attestation_duties_queue != [] 
+            && (
+                || process.attestation_duties_queue[0].slot in process.future_att_consensus_instances_already_decided
+                || !process.current_attestation_duty.isPresent()
+            )    
+        {
+            if process.attestation_duties_queue[0].slot in process.future_att_consensus_instances_already_decided.Keys
+            {
+                var queue_head := process.attestation_duties_queue[0];
+                var new_attestation_slashing_db := f_update_attestation_slashing_db(process.attestation_slashing_db, process.future_att_consensus_instances_already_decided[queue_head.slot]);
+                var s_mod := process.(
+                    attestation_duties_queue := process.attestation_duties_queue[1..],
+                    future_att_consensus_instances_already_decided := process.future_att_consensus_instances_already_decided - {queue_head.slot},
+                    attestation_slashing_db := new_attestation_slashing_db,
+                    attestation_consensus_engine_state := updateConsensusInstanceValidityCheck(
+                        process.attestation_consensus_engine_state,
+                        new_attestation_slashing_db
+                    )                        
+                );
+
+                if  && |s_mod.attestation_duties_queue| > 0 
+                    &&   !s_mod.current_attestation_duty.isPresent()
+                {
+                  
+                    forall an |
+                        && an in dvn.sequence_attestation_duties_to_be_served.Values 
+                        && an.node == n 
+                        && an.attestation_duty.slot < s_mod.attestation_duties_queue[0].slot
+                    ensures 
+                        var slot := an.attestation_duty.slot;
+                        && dvn.consensus_on_attestation_data[slot].decided_value.isPresent()
+                        && construct_SlashingDBAttestation_from_att_data(dvn.consensus_on_attestation_data[slot].decided_value.safe_get()) in s_mod.attestation_slashing_db     
+                    ;                          
+                    {
+                        var slot := an.attestation_duty.slot;
+                   
+                        if an.attestation_duty.slot < process.attestation_duties_queue[0].slot  
+                        {
+                            assert 
+                                && dvn.consensus_on_attestation_data[slot].decided_value.isPresent()
+                                && construct_SlashingDBAttestation_from_att_data(dvn.consensus_on_attestation_data[slot].decided_value.safe_get()) in s_mod.attestation_slashing_db     
+                            ;
+                        }
+                        else 
+                        {
+                            var t :|  dvn.sequence_attestation_duties_to_be_served[t] == an;
+                            assert process.attestation_duties_queue[0] in process.attestation_duties_queue;
+                            var i :|  
+                                    && dvn.sequence_attestation_duties_to_be_served[i].node == n 
+                                    && dvn.sequence_attestation_duties_to_be_served[i].attestation_duty == process.attestation_duties_queue[0];
+                            assert process.attestation_duties_queue[1] in process.attestation_duties_queue;
+                            var j :|  
+                                    && dvn.sequence_attestation_duties_to_be_served[j].node == n 
+                                    && dvn.sequence_attestation_duties_to_be_served[j].attestation_duty == process.attestation_duties_queue[1];   
+
+                            lemma_inv_attestation_duty_queue_is_ordered_3_body_body(
+                                dvn,
+                                n,
+                                process,
+                                1,
+                                i,
+                                j,
+                                t
+                            ); 
+
+                        
+                            assert 
+                                && dvn.consensus_on_attestation_data[slot].decided_value.isPresent()
+                                && construct_SlashingDBAttestation_from_att_data(dvn.consensus_on_attestation_data[slot].decided_value.safe_get()) in s_mod.attestation_slashing_db     
+                            ;
+                            
+                        }
+                    }                  
+                }
+                assert inv_g_a_ii_a_body_body(dvn, n, s_mod);
+
+                forall i: nat, k, l, t  |
+                    inv_attestation_duty_queue_is_ordered_3_body_body_premise(
+                        dvn,
+                        n, 
+                        s_mod,
+                        i,
+                        k, 
+                        l, 
+                        t
+                    )
+                ensures 
+                    s_mod.attestation_duties_queue[i-1].slot == dvn.sequence_attestation_duties_to_be_served[t].attestation_duty.slot      
+                {
+                    assert process.attestation_duties_queue != [];
+                    assert i > 0;
+                    lemma_on_first_seq_element_elimination(process.attestation_duties_queue, s_mod.attestation_duties_queue, i);
+                    // assert i - 1 >= 0;
+                    lemma_on_first_seq_element_elimination(process.attestation_duties_queue, s_mod.attestation_duties_queue, i-1);
+                    // assert s_mod.attestation_duties_queue[i-1] == process.attestation_duties_queue[i]; 
+                    assert inv_attestation_duty_queue_is_ordered_3_body_body_premise(
+                        dvn,
+                        n, 
+                        process,
+                        i+1,
+                        k, 
+                        l, 
+                        t                        
+                    );
+                }   
+
+                forall ad  |
+                    && ad in s_mod.attestation_duties_queue
+                ensures ad in process.attestation_duties_queue
+                {
+                    var i :| 0 <= i < |s_mod.attestation_duties_queue|
+                                && s_mod.attestation_duties_queue[i] == ad;
+                    assert ad in process.attestation_duties_queue;
+                }
+                    // ::
+                    // exists i: nat :: 
+                    //     && i < index_next_attestation_duty_to_be_served
+                    //     && var an := dvn.sequence_attestation_duties_to_be_served[i];
+                    //     && an.attestation_duty == ad
+                    //     && an.node == n                       
+
+                lemma_pred_4_1_b_new_f_check_for_next_queued_duty(s_mod, s', dvn, n , index_next_attestation_duty_to_be_served);
+            }
+            else 
+            {
+                var new_process := process.(
+                    attestation_duties_queue := process.attestation_duties_queue[1..]
+                );   
+
+                var queue_head := process.attestation_duties_queue[0];       
+
+                assert get_upperlimit_decided_instances(s') == s'.latest_attestation_duty.safe_get().slot;
+
+                if process.latest_attestation_duty.isPresent()
+                {
+                    assert inv_g_b_body_body_new(dvn, n, s');
+                }
+                else 
+                {
+                    assert inv_g_b_body_body_new(dvn, n, s');
+                }
+
+                
+            }
+        } 
+        else 
+        {
+            assert inv_g_b_body_body_new(dvn, n, s');
+        }       
+    }    
+
+    lemma lemma_pred_4_1_b_new_helper_transpose_to_new_s_1(
+        s: DVState,
+        event: DV.Event,
+        s': DVState,
+        s_node: DVCNodeState,
+        n: BLSPubkey
+    )
+    requires NextEvent(s, event, s')    
+    requires inv_g_a_ii_a_body_body(s, n, s_node)
+    requires invNetwork(s)
+    requires inv1(s)
+    requires inv3(s)
+    requires inv53(s)  
+    ensures inv_g_a_ii_a_body_body(s', n, s_node)        
+    {
+        assert s'.index_next_attestation_duty_to_be_served <= s'.index_next_attestation_duty_to_be_served <= s'.index_next_attestation_duty_to_be_served + 1;
+
+        if 
+            &&  |s_node.attestation_duties_queue| > 0 
+            &&   !s_node.current_attestation_duty.isPresent()   
+        {
+            forall an |
+                && an in s'.sequence_attestation_duties_to_be_served.Values 
+                && an.node == n 
+                && an.attestation_duty.slot < s_node.attestation_duties_queue[0].slot
+            ensures 
+                var slot := an.attestation_duty.slot;
+                && s'.consensus_on_attestation_data[slot].decided_value.isPresent()
+                && construct_SlashingDBAttestation_from_att_data(s'.consensus_on_attestation_data[slot].decided_value.safe_get()) in s_node.attestation_slashing_db                
+            {
+                var slot := an.attestation_duty.slot;
+                lemma_pred_4_1_g_iii_helper2(s, event, s', slot);
+
+                assert
+                    && s.consensus_on_attestation_data[slot].decided_value.isPresent()
+                    && construct_SlashingDBAttestation_from_att_data(s.consensus_on_attestation_data[slot].decided_value.safe_get()) in s_node.attestation_slashing_db
+                    ;                        
+
+                assert
+                    && s'.consensus_on_attestation_data[slot].decided_value.isPresent();
+                assert
+                    && construct_SlashingDBAttestation_from_att_data(s'.consensus_on_attestation_data[slot].decided_value.safe_get()) in s_node.attestation_slashing_db
+                    ;                      
+
+            }            
+        }     
+        
+    }    
+
+    lemma lemma_pred_4_1_b_new_helper_transpose_to_new_s_2(
+        s: DVState,
+        event: DV.Event,
+        s': DVState,
+        s_node: DVCNodeState,
+        n: BLSPubkey
+    )
+    requires NextEvent(s, event, s')    
+    requires inv_g_a_iii_body_body(s, n, s_node, s.index_next_attestation_duty_to_be_served)
+    requires invNetwork(s)
+    requires inv1(s)
+    requires inv3(s)
+    requires inv53(s)  
+    ensures inv_g_a_iii_body_body(s', n, s_node, s.index_next_attestation_duty_to_be_served)        
+    {
+        assert s'.index_next_attestation_duty_to_be_served <= s'.index_next_attestation_duty_to_be_served <= s'.index_next_attestation_duty_to_be_served + 1;
+
+        assert s.sequence_attestation_duties_to_be_served == s'.sequence_attestation_duties_to_be_served;
+
+        if 
+            &&  |s_node.attestation_duties_queue| == 0 
+            &&   !s_node.current_attestation_duty.isPresent()   
+        {
+            forall i:nat  |
+                && i < s.index_next_attestation_duty_to_be_served
+                && var an := s'.sequence_attestation_duties_to_be_served[i];
+                && an.node == n 
+            ensures 
+                && var an := s'.sequence_attestation_duties_to_be_served[i];
+                var slot := an.attestation_duty.slot;
+                && s'.consensus_on_attestation_data[slot].decided_value.isPresent()
+                && construct_SlashingDBAttestation_from_att_data(s'.consensus_on_attestation_data[slot].decided_value.safe_get()) in s_node.attestation_slashing_db            
+            {
+                var an := s'.sequence_attestation_duties_to_be_served[i];
+                var slot := an.attestation_duty.slot;
+                assert && s.consensus_on_attestation_data[slot].decided_value.isPresent();
+                lemma_pred_4_1_g_iii_helper2(s, event, s', slot);
+
+                assert
+                    && s.consensus_on_attestation_data[slot].decided_value.isPresent()
+                    && construct_SlashingDBAttestation_from_att_data(s.consensus_on_attestation_data[slot].decided_value.safe_get()) in s_node.attestation_slashing_db
+                    ;                        
+
+                assert
+                    && s'.consensus_on_attestation_data[slot].decided_value.isPresent();
+                assert
+                    && construct_SlashingDBAttestation_from_att_data(s'.consensus_on_attestation_data[slot].decided_value.safe_get()) in s_node.attestation_slashing_db
+                    ;                      
+
+            }            
+        }     
+        
+    }         
+
+    lemma lemma_pred_4_1_b_new_helper_transpose_to_new_s_3(
+        s: DVState,
+        event: DV.Event,
+        s': DVState,
+        s_node: DVCNodeState,
+        n: BLSPubkey
+    )
+    requires NextEvent(s, event, s')    
+    requires inv_attestation_duty_queue_is_ordered_3_body_body(s, n, s_node)
+    requires inv_attestation_duty_queue_is_ordered_4_body_body(s, n, s_node, s.index_next_attestation_duty_to_be_served)    
+
+    ensures inv_attestation_duty_queue_is_ordered_3_body_body(s', n, s_node)    
+    ensures inv_attestation_duty_queue_is_ordered_4_body_body(s', n, s_node, s.index_next_attestation_duty_to_be_served)    
+     
+    {
+
+        assert s.sequence_attestation_duties_to_be_served == s'.sequence_attestation_duties_to_be_served;
+
+        forall i, k, l, t  |
+            inv_attestation_duty_queue_is_ordered_3_body_body_premise(
+                s',
+                n, 
+                s_node,
+                i,
+                k, 
+                l, 
+                t
+            )
+        ensures
+            s_node.attestation_duties_queue[i-1].slot == s'.sequence_attestation_duties_to_be_served[t].attestation_duty.slot     
+        {
+            assert
+            inv_attestation_duty_queue_is_ordered_3_body_body_premise(
+                s,
+                n, 
+                s_node,
+                i,
+                k, 
+                l, 
+                t
+            );
+
+        }  
+
+        if |s_node.attestation_duties_queue| > 0
+        {
+            forall i |
+                inv_attestation_duty_queue_is_ordered_4_body_body_premise(
+                    s',
+                    n, 
+                    s_node,
+                    i,
+                    s.index_next_attestation_duty_to_be_served
+                )
+            ensures
+                var last := s_node.attestation_duties_queue[|s_node.attestation_duties_queue|-1];
+                last.slot == s'.sequence_attestation_duties_to_be_served[i].attestation_duty.slot
+            {
+                assert
+                inv_attestation_duty_queue_is_ordered_4_body_body_premise(
+                    s,
+                    n, 
+                    s_node,
+                    i,
+                    s.index_next_attestation_duty_to_be_served
+                )
+                ;
+            }
+        } 
+     
+    }      
+
+    lemma lemma_pred_4_1_b_new_helper_transpose_to_new_s_4(
+        s: DVState,
+        event: DV.Event,
+        s': DVState,
+        s_node: DVCNodeState,
+        n: BLSPubkey
+    )
+    requires NextEvent(s, event, s')    
+    requires inv_g_a_iv_a_body_body(s, n, s_node)
+    requires invNetwork(s)
+    requires inv1(s)
+    requires inv3(s)
+    requires inv53(s)  
+    ensures inv_g_a_iv_a_body_body(s', n, s_node)        
+    {
+        assert s'.index_next_attestation_duty_to_be_served <= s'.index_next_attestation_duty_to_be_served <= s'.index_next_attestation_duty_to_be_served + 1;
+
+        assert s.sequence_attestation_duties_to_be_served == s'.sequence_attestation_duties_to_be_served;
+
+        if 
+            &&  |s_node.attestation_duties_queue| > 0 
+            &&   s_node.latest_attestation_duty.isPresent()
+        {
+            forall an |
+                && an in s'.sequence_attestation_duties_to_be_served.Values 
+                && an.node == n 
+                && s_node.latest_attestation_duty.safe_get().slot < an.attestation_duty.slot < s_node.attestation_duties_queue[0].slot
+            ensures 
+                var slot := an.attestation_duty.slot;
+                && s'.consensus_on_attestation_data[slot].decided_value.isPresent()
+                && construct_SlashingDBAttestation_from_att_data(s'.consensus_on_attestation_data[slot].decided_value.safe_get()) in s_node.attestation_slashing_db          
+            {
+                var slot := an.attestation_duty.slot;
+
+                assert && s.consensus_on_attestation_data[slot].decided_value.isPresent();
+                lemma_pred_4_1_g_iii_helper2(s, event, s', slot);
+
+                assert
+                    && s.consensus_on_attestation_data[slot].decided_value.isPresent()
+                    && construct_SlashingDBAttestation_from_att_data(s.consensus_on_attestation_data[slot].decided_value.safe_get()) in s_node.attestation_slashing_db
+                    ;                        
+
+                assert
+                    && s'.consensus_on_attestation_data[slot].decided_value.isPresent();
+                assert
+                    && construct_SlashingDBAttestation_from_att_data(s'.consensus_on_attestation_data[slot].decided_value.safe_get()) in s_node.attestation_slashing_db
+                    ;                      
+
+            }            
+        }     
+        
+    }            
+
+    lemma lemma_pred_4_1_b_new_helper_transpose_to_new_s_multiple(
+        s: DVState,
+        event: DV.Event,
+        s': DVState,
+        s_node: DVCNodeState,
+        n: BLSPubkey
+    )
+    requires NextEvent(s, event, s')    
+    requires inv_g_iii_b_body_body(s, n, s_node, s.index_next_attestation_duty_to_be_served)
+    // requires inv_attestation_duty_queue_is_ordered_3_body_body(s, n, s_node)
+    // requires inv_attestation_duty_queue_is_ordered_4_body_body(s, n, s_node, s.index_next_attestation_duty_to_be_served)
+
+    ensures inv_g_iii_b_body_body(s', n, s_node, s.index_next_attestation_duty_to_be_served)
+    // ensures inv_attestation_duty_queue_is_ordered_3_body_body(s', n, s_node)
+    // ensures inv_attestation_duty_queue_is_ordered_4_body_body(s', n, s_node, s.index_next_attestation_duty_to_be_served)
+    {
+        assert s'.index_next_attestation_duty_to_be_served <= s'.index_next_attestation_duty_to_be_served <= s'.index_next_attestation_duty_to_be_served + 1;
+        
+    }   
+
+    lemma lemma_pred_4_1_b_new_helper_easy(
+        s: DVState,
+        event: DV.Event,
+        s_node: DVCNodeState,
+        s'_node: DVCNodeState,
+        n: BLSPubkey
+    )
+    requires inv_g_b_body_body_new(s, n, s_node)
+    requires s_node.latest_attestation_duty == s'_node.latest_attestation_duty
+    requires s_node.current_attestation_duty == s'_node.current_attestation_duty
+    requires s_node.attestation_slashing_db <= s'_node.attestation_slashing_db
+    ensures inv_g_b_body_body_new(s, n, s'_node)        
+    {
+        assert get_upperlimit_decided_instances(s'_node) == get_upperlimit_decided_instances(s_node);
+
+        forall an |
+            && an in s.sequence_attestation_duties_to_be_served.Values 
+            && an.node == n 
+            && an.attestation_duty.slot < get_upperlimit_decided_instances(s'_node)     
+        ensures 
+                var slot := an.attestation_duty.slot;
+                && s.consensus_on_attestation_data[slot].decided_value.isPresent()
+                && construct_SlashingDBAttestation_from_att_data(s.consensus_on_attestation_data[slot].decided_value.safe_get()) in s'_node.attestation_slashing_db                   
+        {
+            var slot := an.attestation_duty.slot;
+
+            assert && s.consensus_on_attestation_data[slot].decided_value.isPresent();
+
+            assert
+                && construct_SlashingDBAttestation_from_att_data(s.consensus_on_attestation_data[slot].decided_value.safe_get()) in s_node.attestation_slashing_db
+                ;     
+
+            assert
+                && construct_SlashingDBAttestation_from_att_data(s.consensus_on_attestation_data[slot].decided_value.safe_get()) in s'_node.attestation_slashing_db
+                ;                                         
+                    
+        }            
+  
+        
+    }        
+
+    predicate lemma_pred_4_1_b_new_precond(s: DVState) 
+    {
+        && inv1(s)
+        && inv2(s)
+        && inv3(s)
+        && inv53(s)    
+        && invNetwork(s)
+        && pred_4_1_g_b_new(s) //
+        && inv_g_a_ii_a(s) //
+        && pred_4_1_g_iii_b(s) //
+        && inv_g_d_a(s) //
+        && inv_attestation_duty_queue_is_ordered_3(s) //  
+        && inv_attestation_duty_queue_is_ordered_4(s) //    
+        && inv_g_a_iii(s) //
+        && inv_g_a_iv(s) //
+        && pred_4_1_b(s) //
+        && pred_4_1_c(s) //  
+        && is_sequence_attestation_duties_to_be_served_orderd(s) //
+        && pred_inv_current_latest_attestation_duty_match(s)
+
+
+        && pred_4_1_g_iii(s) 
+
+        && construct_signed_attestation_signature_assumptions_helper(
+            s.construct_signed_attestation_signature,
+            s.dv_pubkey,
+            s.all_nodes
+        )    
+        && pred_rcvd_attestation_shares_is_in_all_messages_sent(s) 
+        && pred_4_1_f_b(s)
+        && inv_attestation_shares_to_broadcast_is_a_subset_of_all_messages_sent(s)      
+        && pred_4_1_f_a(s)    
+        && pred_4_1_g_i(s)    
+        && pred_4_1_g_i_for_dvc(s)         
+    }
+
+    lemma lemma_pred_4_1_b_new_helper_summary(
+        s: DVState,
+        event: DV.Event,
+        s': DVState        
+    )
+    requires NextEvent(s, event, s')
+    requires event.HonestNodeTakingStep?
+    requires lemma_pred_4_1_b_new_precond(s)
+    {
+        assert s.att_network.allMessagesSent <= s'.att_network.allMessagesSent;
+        match event 
+        {
+            
+            case HonestNodeTakingStep(node, nodeEvent, nodeOutputs) =>
+                var s_node := s.honest_nodes_states[node];
+                var s'_node := s'.honest_nodes_states[node];
+                lemma_pred_4_1_g_iii_helper3a(s, event, s', s_node, node);
+                lemma_pred_4_1_g_iii_helper3c(s, event, s', s_node, node);
+                lemma_pred_4_1_b_new_helper_transpose_to_new_s_1(s, event, s', s_node, node);
+                lemma_pred_4_1_b_new_helper_transpose_to_new_s_2(s, event, s', s_node, node);
+                lemma_pred_4_1_b_new_helper_transpose_to_new_s_3(s, event, s', s_node, node);
+                lemma_pred_4_1_b_new_helper_transpose_to_new_s_4(s, event, s', s_node, node);
+
+                lemma_pred_4_1_b_new_helper_transpose_to_new_s_multiple(s, event, s', s_node, node);
+
+                // lemma_pred_4_1_b(s, event, s');
+                // lemma_pred_4_1_c(s, event, s');
+
+                lemma_inv_sequence_attestation_duties_to_be_served_orderd(s, event, s');
+
+                // assert inv_g_b_body_body_new(s', node, s_node);
+                // assert inv_g_d_a_body_body(s', node, s_node);
+                // assert inv_g_a_ii_a_body_body(s', node, s_node);
+                // assert inv_g_iii_b_body_body(s', node, s_node, s.index_next_attestation_duty_to_be_served);
+                // assert inv_g_a_iii_body_body(s', node, s_node, s.index_next_attestation_duty_to_be_served);
+                // assert inv_attestation_duty_queue_is_ordered_3_body_body(s', node, s_node);
+                // assert inv_attestation_duty_queue_is_ordered_4_body_body(s', node, s_node, s.index_next_attestation_duty_to_be_served);
+                // assert pred_4_1_b(s');
+                // assert pred_4_1_c(s');             
+                // assert inv_g_a_iv_a_body_body(s', node, s_node);
+        }        
+    }   
+
+    lemma lemma_ServeAttstationDuty(
+        s: DVState,
+        event: DV.Event,
+        s': DVState
+    )
+    requires NextEvent(s, event, s')    
+    requires event.HonestNodeTakingStep?
+    requires event.event.ServeAttstationDuty?
+    ensures
+                        var attestation_duty := event.event.attestation_duty;
+                        var an := s'.sequence_attestation_duties_to_be_served[s'.index_next_attestation_duty_to_be_served - 1];
+
+                        && attestation_duty == an.attestation_duty
+                        && event.node == an.node    
+    {
+        assert s.att_network.allMessagesSent <= s'.att_network.allMessagesSent;
+        match event 
+        {
+            
+            case HonestNodeTakingStep(node, nodeEvent, nodeOutputs) =>
+                var s_node := s.honest_nodes_states[node];
+                var s'_node := s'.honest_nodes_states[node];
+
+
+                match nodeEvent
+                {
+                    case ServeAttstationDuty(attestation_duty) => 
+                        assert s.sequence_attestation_duties_to_be_served == s'.sequence_attestation_duties_to_be_served;
+                        assert s.index_next_attestation_duty_to_be_served == s'.index_next_attestation_duty_to_be_served - 1;
+
+                        var an := s'.sequence_attestation_duties_to_be_served[s'.index_next_attestation_duty_to_be_served - 1];
+
+                        assert attestation_duty == an.attestation_duty;
+                        assert node == an.node;
+
+                }
+        }        
+    }
+    
+    lemma lemma_pred_4_1_b_new(
+        s: DVState,
+        event: DV.Event,
+        s': DVState
+    )
+    requires NextEvent(s, event, s')
+    requires lemma_pred_4_1_b_new_precond(s)
+  
+
+
+    ensures pred_4_1_g_b_new(s');  
+    {
+        assert s.att_network.allMessagesSent <= s'.att_network.allMessagesSent;
+        match event 
+        {
+            
+            case HonestNodeTakingStep(node, nodeEvent, nodeOutputs) =>
+                var s_node := s.honest_nodes_states[node];
+                var s'_node := s'.honest_nodes_states[node];
+                lemma_pred_4_1_g_iii_helper3a(s, event, s', s_node, node);
+                lemma_pred_4_1_g_iii_helper3c(s, event, s', s_node, node);
+                lemma_pred_4_1_b_new_helper_transpose_to_new_s_1(s, event, s', s_node, node);
+                lemma_pred_4_1_b_new_helper_transpose_to_new_s_2(s, event, s', s_node, node);
+                lemma_pred_4_1_b_new_helper_transpose_to_new_s_3(s, event, s', s_node, node);
+                lemma_pred_4_1_b_new_helper_transpose_to_new_s_4(s, event, s', s_node, node);
+
+                lemma_pred_4_1_b_new_helper_transpose_to_new_s_multiple(s, event, s', s_node, node);
+
+                lemma_pred_4_1_b(s, event, s');
+                lemma_pred_4_1_c(s, event, s');
+
+                lemma_inv_sequence_attestation_duties_to_be_served_orderd(s, event, s');
+
+                assert inv_g_b_body_body_new(s', node, s_node);
+                assert inv_g_d_a_body_body(s', node, s_node);
+                assert inv_g_a_ii_a_body_body(s', node, s_node);
+                assert inv_g_iii_b_body_body(s', node, s_node, s.index_next_attestation_duty_to_be_served);
+                assert inv_g_a_iii_body_body(s', node, s_node, s.index_next_attestation_duty_to_be_served);
+                assert inv_attestation_duty_queue_is_ordered_3_body_body(s', node, s_node);
+                assert inv_attestation_duty_queue_is_ordered_4_body_body(s', node, s_node, s.index_next_attestation_duty_to_be_served);
+                assert pred_4_1_b(s');
+                assert pred_4_1_c(s');             
+                assert inv_g_a_iv_a_body_body(s', node, s_node);
+                assert is_sequence_attestation_duties_to_be_served_orderd(s');
+
+                match nodeEvent
+                {
+                    case ServeAttstationDuty(attestation_duty) => 
+                        assert s.index_next_attestation_duty_to_be_served == s'.index_next_attestation_duty_to_be_served - 1;
+                        lemma_ServeAttstationDuty(s, event, s');
+                        lemma_pred_4_1_b_new_f_serve_attestation_duty(
+                            s_node,
+                            attestation_duty,
+                            s'_node,
+                            s', 
+                            node,
+                            s'.index_next_attestation_duty_to_be_served
+                        );
+                        assert inv_g_b_body_body_new(s', node, s'_node);                     
+ 
+                              
+
+                
+                    case AttConsensusDecided(id, decided_attestation_data) =>  
+                        assert s.index_next_attestation_duty_to_be_served == s'.index_next_attestation_duty_to_be_served;    
+                        lemma_pred_4_1_g_iii_helper5(s, event, s');                 
+                        lemma_pred_4_1_b_new_f_att_consensus_decided(
+                            s_node,
+                            id,
+                            decided_attestation_data,
+                            s'_node,
+                            s', 
+                            node,
+                            s.index_next_attestation_duty_to_be_served
+                        ); 
+                        assert inv_g_b_body_body_new(s', node, s'_node);                        
+               
+                   
+                    case ReceviedAttesttionShare(attestation_share) => 
+                        lemma_f_listen_for_attestation_shares_constants(s_node, attestation_share, s'_node);
+                        lemma_pred_4_1_b_new_helper_easy(s', event, s_node, s'_node, node );
+                        
+
+                    case ImportedNewBlock(block) => 
+                        var s_node2 := add_block_to_bn(s_node, nodeEvent.block);
+                        lemma2_inv_attestation_duty_queue_is_ordered_3_body_body(s', node, s_node, s_node2);
+                        lemma_pred_4_1_b_new_f_listen_for_new_imported_blocks(
+                            s_node2,
+                            block,
+                            s'_node,
+                            s', 
+                            node,
+                            s.index_next_attestation_duty_to_be_served
+                        );  
+                        assert inv_g_b_body_body_new(s', node, s'_node);                     
+                    
+                 
+                    case ResendAttestationShares => 
+                        lemma_pred_4_1_b_new_helper_easy(s', event, s_node, s'_node, node );
+
+                   
+                    case NoEvent => 
+                        lemma_pred_4_1_b_new_helper_easy(s', event, s_node, s'_node, node );
+                }
+                assert inv_g_b_body_body_new(s', node, s'_node);  
+                
+
+                forall hn |
+                    && hn in s'.honest_nodes_states.Keys   
+                ensures inv_g_b_body_body_new(s', hn, s'.honest_nodes_states[hn]); 
+                {
+                    if hn != node 
+                    {
+                        // lemma_pred_4_1_g_iii_helper3(s, event, s', s.honest_nodes_states[hn]);
+                        assert s.honest_nodes_states[hn] == s'.honest_nodes_states[hn];
+                        lemma_pred_4_1_g_iii_helper3a(s, event, s', s.honest_nodes_states[hn], hn);
+                        lemma_pred_4_1_b_new_helper_easy(s', event, s.honest_nodes_states[hn], s'.honest_nodes_states[hn], hn);
+                        // assert inv_g_b_body_body_new(s', hn, s'.honest_nodes_states[hn]);                        
+                    }
+                }     
+                assert pred_4_1_g_b_new(s');                  
+        
+
+            case AdeversaryTakingStep(node, new_attestation_share_sent, messagesReceivedByTheNode) =>
+                 forall hn |
+                    && hn in s'.honest_nodes_states.Keys   
+                ensures inv_g_b_body_body_new(s', hn, s'.honest_nodes_states[hn]); 
+                {
+
+                    {
+                        // lemma_pred_4_1_g_iii_helper3(s, event, s', s.honest_nodes_states[hn]);
+                        assert s.honest_nodes_states[hn] == s'.honest_nodes_states[hn];
+                        lemma_pred_4_1_g_iii_helper3a(s, event, s', s.honest_nodes_states[hn], hn);
+                        lemma_pred_4_1_b_new_helper_easy(s', event, s.honest_nodes_states[hn], s'.honest_nodes_states[hn], hn);
+                        // assert inv_g_b_body_body_new(s', hn, s'.honest_nodes_states[hn]);                        
+                    }
+                }     
+                assert pred_4_1_g_b_new(s'); 
+
+        }
+    }        
+                
+}
